rustfrontend/Clightgenspec.v
@@ -1,7 +1,7 @@
 Require Import Coqlib Maps Errors Integers Floats.
 Require Import AST Linking Memory.
 Require Import Ctypes Cop Csyntax Clight.
-Require Import Rusttypes RustlightBase RustIR.
+Require Import Rusttypes Rustlight RustIR.
 Require Import Clightgen.
 
 Import ListNotations.
