rustfrontend/RustIRsem.v
@@ -12,7 +12,7 @@ Require Import Smallstep.
 Require Import Ctypes Rusttypes.
 Require Import Cop RustOp.
 Require Import LanguageInterface.
-Require Import Clight RustlightBase RustIR.
+Require Import Clight Rustlight RustIR.
 Require Import InitDomain.
 
 Import ListNotations.
@@ -79,6 +79,13 @@ Inductive state: Type :=
     (ms: members)
     (k: cont)
     (m: mem): state.              
+
+Inductive function_entry (ge: genv) (f: function) (vargs: list val) (m: mem) (e: env) (m': mem) : Prop :=
+| function_entry_intro: forall m1,
+    list_norepet (var_names f.(fn_params) ++ var_names f.(fn_vars)) ->
+    alloc_variables ge empty_env m (f.(fn_params) ++ f.(fn_vars)) e m1 ->
+    bind_parameters ge e m1 f.(fn_params) vargs m' ->
+    function_entry ge f vargs m e m'.
 
 Section SMALLSTEP.
 
