rustfrontend/Rustlight.v
@@ -1,0 +1,370 @@
+Require Import Coqlib.
+Require Import Errors.
+Require Import Maps.
+Require Import Integers.
+Require Import Floats.
+Require Import AST.
+Require Import Ctypes Rusttypes.
+Require Import Cop RustOp.
+
+Local Open Scope error_monad_scope.
+
+(** * High-level Rust-like language  *)
+
+
+(** ** Place (used to build lvalue expression) *)
+
+Inductive place : Type :=
+| Plocal : ident -> type -> place
+| Pfield : place -> ident -> type -> place (**r access a field of struct: p.(id)  *)
+| Pderef : place -> type -> place
+| Pdowncast: place -> ident -> type -> place (**r represent the location of a constructor *)
+.
+
+Lemma place_eq: forall (p1 p2: place), {p1=p2} + {p1<>p2}.
+Proof.
+  generalize type_eq ident_eq. intros.
+  decide equality.
+Qed.
+
+Global Opaque place_eq.
+
+Definition typeof_place p :=
+  match p with
+  | Plocal _ ty => ty
+  | Pfield _ _ ty => ty
+  | Pderef _ ty => ty
+  | Pdowncast _ _ ty => ty
+  end.
+
+
+(** ** Expression *)
+
+Inductive pexpr : Type :=
+| Eunit                                 (**r unit value  *)
+| Econst_int: int -> type -> pexpr       (**r integer literal *)
+| Econst_float: float -> type -> pexpr   (**r double float literal *)
+| Econst_single: float32 -> type -> pexpr (**r single float literal *)
+| Econst_long: int64 -> type -> pexpr    (**r long integer literal *)
+| Eplace: place -> type -> pexpr (**r use of a variable, the only lvalue expression *)
+| Ecktag: place -> ident -> pexpr           (**r check the tag of variant, e.g. [Ecktag p.(fid)]. We cannot check a downcast *)
+| Eref:  origin -> mutkind -> place -> type -> pexpr     (**r &[mut] p  *)
+| Eunop: unary_operation -> pexpr -> type -> pexpr  (**r unary operation *)
+| Ebinop: binary_operation -> pexpr -> pexpr -> type -> pexpr. (**r binary operation *)
+
+(* The evaluaiton of expr may produce a moved-out place *)
+Inductive expr : Type :=
+| Emoveplace: place -> type -> expr
+| Epure: pexpr -> expr.
+
+
+Definition typeof_pexpr (pe: pexpr) : type :=
+  match pe with
+  | Eunit => Tunit
+  | Ecktag _ _ => type_bool
+  | Econst_int _ ty
+  | Econst_float _ ty
+  | Econst_single _ ty
+  | Econst_long _ ty                
+  | Eplace _ ty
+  | Eref _ _ _ ty
+  | Eunop _ _ ty
+  | Ebinop _ _ _ ty => ty
+  end.
+
+Definition typeof (e: expr) : type :=
+  match e with
+  | Emoveplace _ ty => ty
+  | Epure pe => typeof_pexpr pe
+    end.
+
+
+(* What Tbox corresponds to? *)
+(** TODO: Tbox -> None. reference -> None, raw poinetr -> C pointer,
+Option<reference> -> C pointer *)
+Fixpoint to_ctype (ty: type) : Ctypes.type :=
+  match ty with
+  | Tunit => Ctypes.type_int32s  (* unit is set to zero *)
+  (* | Tbox _  => None *)
+  | Tint sz si => Ctypes.Tint sz si noattr
+  | Tlong si => Ctypes.Tlong si noattr
+  | Tfloat fz => Ctypes.Tfloat fz noattr
+  | Tstruct _ id  => Ctypes.Tstruct id noattr
+  (* variant = Struct {tag: .. ; f: union} *)
+  | Tvariant _ id => Ctypes.Tstruct id noattr
+  | Treference _ _ ty
+  | Tbox ty => Tpointer (to_ctype ty) noattr
+      (* match (to_ctype ty) with *)
+      (* | Some ty' =>  *)
+      (*     Some (Ctypes.Tpointer ty' attr) *)
+      (* | _ => None *)
+  (* end *)
+  | Tarray ty sz => Ctypes.Tarray (to_ctype ty) sz noattr
+  | Tfunction _ _ tyl ty cc =>
+      Ctypes.Tfunction (to_ctypelist tyl) (to_ctype ty) cc
+  end
+    
+with to_ctypelist (tyl: typelist) : Ctypes.typelist :=
+       match tyl with
+       | Tnil => Ctypes.Tnil
+       | Tcons ty tyl =>
+           Ctypes.Tcons (to_ctype ty) (to_ctypelist tyl)
+       end.
+                                  
+
+Inductive statement : Type :=
+| Sskip : statement                   (**r do nothing *)
+| Slet : ident -> type -> statement -> statement (**r declare a variable. let ident: type in *)
+| Sassign : place -> expr -> statement (**r assignment [place' = rvalue]. Downcast cannot appear in LHS *)
+| Sassign_variant : place -> ident -> ident -> expr -> statement (**r assign variant to a place *)
+| Sbox: place -> expr -> statement        (**r box assignment [place = Box::new(expr)]  *)
+| Scall: place -> expr -> list expr -> statement (**r function call, p =
+  f(...). The assignee is mandatory, because we need to ensure that
+  the return value (may be a box) is received *)
+| Ssequence : statement -> statement -> statement  (**r sequence *)
+| Sifthenelse : expr  -> statement -> statement -> statement (**r conditional *)
+| Sloop: statement -> statement (**r infinite loop *)
+| Sbreak : statement                      (**r [break] statement *)
+| Scontinue : statement                   (**r [continue] statement *)
+| Sreturn : option expr -> statement.      (**r [return] statement *)
+
+
+Record function : Type := mkfunction {
+  fn_generic_origins : list origin;
+  fn_origins_relation: list (origin * origin);
+  fn_drop_glue : option ident;
+  fn_return: type;
+  fn_callconv: calling_convention;
+  fn_params: list (ident * type);
+  fn_body: statement
+}.
+
+Definition var_names (vars: list(ident * type)) : list ident :=
+  List.map (@fst ident type) vars.
+
+(* Used in Rustlightown and RustIRgen *)
+Fixpoint extract_vars (stmt: Rustlight.statement) : list (ident * type) :=
+  match stmt with
+  | Slet id ty s =>
+      (id,ty) :: extract_vars s
+  | Rustlight.Ssequence s1 s2 =>
+      extract_vars s1 ++ extract_vars s2
+  | Rustlight.Sifthenelse _ s1 s2 =>
+      extract_vars s1 ++ extract_vars s2
+  | Rustlight.Sloop s =>
+      extract_vars s
+  | _ => nil
+  end.
+
+Definition fundef := Rusttypes.fundef function.
+
+Definition program := Rusttypes.program function.
+
+Fixpoint type_of_params (params: list (ident * type)) : typelist :=
+  match params with
+  | nil => Tnil
+  | (id, ty) :: rem => Tcons ty (type_of_params rem)
+  end.
+
+
+Definition type_of_function (f: function) : type :=
+  Tfunction (fn_generic_origins f) (fn_origins_relation f) (type_of_params (fn_params f)) (fn_return f) (fn_callconv f).
+
+Definition type_of_fundef (f: fundef) : type :=
+  match f with
+  | Internal fd => type_of_function fd
+  | External orgs org_rels ef typs typ cc =>
+      Tfunction orgs org_rels typs typ cc
+  end.
+
+(** Prefix of a place  *)
+
+Fixpoint parent_paths (p: place) : list place :=
+  match p with
+  | Plocal _ _ => nil
+  | Pfield p' _ _ => p' :: parent_paths p'
+  | Pderef p' _ =>  p' :: parent_paths p'
+  | Pdowncast p' _ _ => p' :: parent_paths p'
+  end.
+
+Fixpoint shallow_parent_paths (p: place) : list place :=
+  match p with
+  | Plocal _ _ => nil
+  | Pfield p' _ _ => p' :: shallow_parent_paths p'
+  | Pderef _ _ => nil
+  (** FIXMEL: how to handle downcast? *)
+  | Pdowncast p' _ _ => p' :: shallow_parent_paths p'
+  end.
+
+Fixpoint support_parent_paths (p: place) : list place :=
+  match p with
+  | Plocal _ _ => nil
+  | Pfield p' _ _ => p' :: support_parent_paths p'
+  | Pderef p' _ =>
+      match typeof_place p' with
+      | Tbox _ 
+      | Treference _ Mutable _ =>
+          p' :: support_parent_paths p'
+      | _ => nil
+      end
+  | Pdowncast p' _ _ => p' :: support_parent_paths p'
+  end.
+
+
+Definition is_prefix (p1 p2: place) : bool :=
+  place_eq p1 p2 || in_dec place_eq p1 (parent_paths p2).
+
+Definition is_shallow_prefix (p1 p2: place) : bool :=
+  place_eq p1 p2 || in_dec place_eq p1 (shallow_parent_paths p2).
+
+Definition is_support_prefix (p1 p2: place) : bool :=
+  place_eq p1 p2 || in_dec place_eq p1 (support_parent_paths p2).
+
+Definition is_prefix_strict (p1 p2: place) : bool :=
+  in_dec place_eq p1 (parent_paths p2).
+
+Lemma is_prefix_strict_trans p1 p2 p3:
+  is_prefix_strict p1 p2 = true ->
+  is_prefix_strict p2 p3 = true ->
+  is_prefix_strict p1 p3 = true.
+Admitted.
+
+Lemma is_prefix_refl: forall p, is_prefix p p = true.
+Admitted.
+
+
+Lemma is_prefix_trans: forall p1 p2 p3, is_prefix p1 p2 = true -> is_prefix p2 p3 = true -> is_prefix p1 p3 = true.
+Admitted.
+
+
+Fixpoint local_of_place (p: place) :=
+  match p with
+  | Plocal id _ => id
+  | Pfield p' _ _ => local_of_place p'
+  | Pderef p' _ => local_of_place p'
+  | Pdowncast p' _ _ => local_of_place p'
+  end.
+
+Definition is_sibling (p1 p2: place) : bool :=
+  Pos.eqb (local_of_place p1) (local_of_place p2)
+  && negb (is_prefix p1 p2 && is_prefix p2 p1).
+
+Fixpoint local_type_of_place (p: place) :=
+  match p with
+  | Plocal id ty => ty
+  | Pfield p' ty _ => local_type_of_place p'
+  | Pderef p' ty => local_type_of_place p'
+  | Pdowncast p' _ _ => local_type_of_place p'
+  end.
+  
+
+(** Classify function (copy from Cop.v)  *)
+Inductive classify_fun_cases : Type :=
+| fun_case_f (targs: typelist) (tres: type) (cc: calling_convention) (**r (pointer to) function *)
+| fun_default.
+
+Definition classify_fun (ty: type) :=
+  match ty with
+  | Tfunction _ _ args res cc => fun_case_f args res cc
+  (** TODO: do we allow function pointer?  *)
+  (* | Treference (Tfunction args res cc) _ => fun_case_f args res cc *)
+  | _ => fun_default
+  end.
+  
+
+(** ** Notations of Rustlight program *)
+
+Declare Custom Entry rustlight.
+Declare Scope rustlight_scope.
+Declare Custom Entry rustlight_aux.
+Declare Custom Entry rustlight_place.
+Declare Custom Entry rustlight_expr.
+
+Notation "<{ s }>" := s (s custom rustlight_aux) : rustlight_scope.
+Notation "s" := s (in custom rustlight_aux at level 0, s custom rustlight) : rustlight_scope.
+
+(* Notations for statement (level > 50) *)
+Notation "'if' e 'then' s1 'else' s2 'end'" := (Sifthenelse e s1 s2) (in custom rustlight at level 80, e custom rustlight_expr at level 20, s1 at level 99, s2 at level 99) : rustlight_scope.
+Notation "s1 ; s2" := (Ssequence s1 s2) (in custom rustlight at level 99, right associativity) : rustlight_scope.
+Notation "'skip'" := Sskip (in custom rustlight at level 0) : rustlight_scope.
+Notation "'break'" := Sbreak (in custom rustlight at level 0) : rustlight_scope.
+Notation "'continue'" := Scontinue (in custom rustlight at level 0) : rustlight_scope.
+Notation "'return0'" := (Sreturn None) (in custom rustlight at level 0) : rustlight_scope.
+Notation "'return' e" := (Sreturn (@Some expr e)) (in custom rustlight at level 80, e custom rustlight_expr at level 20) : rustlight_scope.
+Notation "'let' x : t 'in' s 'end' " := (Slet x t s) (in custom rustlight at level 80, s at level 99, x global, t global) : rustlight_scope.
+Notation "'loop' s 'end'" := (Sloop s) (in custom rustlight at level 80, s at level 99) : rustlight_scope.
+Notation "'Box' p := ( e ) " := (Sbox p e) (in custom rustlight at level 80, p custom rustlight_place at level 20, e custom rustlight_expr at level 20) : rustlight_scope.
+Notation " p := e " := (Sassign p e) (in custom rustlight at level 80, p custom rustlight_place at level 20, e custom rustlight_expr at level 20) : rustlight_scope.
+Notation " p <- f @ l " := (Scall p f l) (in custom rustlight at level 80, p custom rustlight_place at level 20, f custom rustlight_expr at level 20, l custom rustlight_expr at level 20) : rustlight_scope.
+
+
+(* Notation for place *)
+
+Notation " ( x ) " := x (in custom rustlight_place at level 20) : rustlight_scope.
+Notation " x # t " := (Plocal x t) (in custom rustlight_place at level 0, x global, t global) : rustlight_scope.
+Notation " ! p " := (Pderef p (deref_type (typeof_pexpr p))) (in custom rustlight_place at level 10, p at level 20) : rustlight_scope.
+Notation " p . x < t > " := (Pfield p x t) (in custom rustlight_place at level 10, x global, t global) : rustlight_scope.
+
+
+(* Notations for expression. Expression is at level 20 *)
+
+Notation " ( x ) " := x (in custom rustlight_expr at level 20) : rustlight_scope.
+Notation " { x , .. , y } " := (cons x .. (cons y nil) .. ) (in custom rustlight_expr at level 20) : rustlight_scope.
+Notation " e1 < e2 " := ((Ebinop Ole e1 e2 type_bool)) (in custom rustlight_expr at level 15, e2 at level 20, left associativity) : rustlight_scope.
+Notation " $ k " := ((Econst_int (Int.repr k) type_int32s)) (in custom rustlight_expr at level 10, k constr) : rustlight_scope.
+Notation " e1 * e2 " := ((Ebinop Omul e1 e2 (typeof e1)))  (in custom rustlight_expr at level 15, e2 at level 20, left associativity) : rustlight_scope.
+Notation " e1 - e2 " := ((Ebinop Osub e1 e2 (typeof e1)))  (in custom rustlight_expr at level 15, e2 at level 20, left associativity) : rustlight_scope.
+Notation " 'copy' p " := ((Eplace p (typeof_place p))) (in custom rustlight_expr at level 20, p custom rustlight_place at level 20) : rustlight_scope.
+Notation " 'move' p " := (Emoveplace p (typeof_place p)) (in custom rustlight_expr at level 20, p custom rustlight_place at level 20) : rustlight_scope.
+(* TODO: Ecktag and Eget/Emoveget *)
+
+
+(* Print Grammar constr. *)
+
+Local Open Scope rustlight_scope.
+
+Definition A : ident := 1%positive.
+Definition B : ident := 2%positive.
+Definition C : ident := 3%positive.
+Definition D : ident := 4%positive.
+Definition E : ident := 5%positive.
+
+
+(* Print Custom Grammar rustlight. *)
+
+Definition ident_to_place_int32s (id: ident) : place := Plocal id type_int32s.
+
+Definition place_to_pexpr (p: place) : pexpr := (Eplace p (typeof_place p)).
+
+Definition pexpr_to_expr (pe: pexpr) : expr := Epure pe.
+
+Coercion ident_to_place_int32s : ident >-> place.
+Coercion place_to_pexpr: place >-> pexpr.
+Coercion pexpr_to_expr: pexpr >-> expr.
+
+Fail Definition test_option_ident_to_expr : option expr  := Some A.
+Definition test_option_ident_to_expr : option expr  := @Some expr A.
+
+(* Print Graph. *)
+(* Print Coercion Paths ident expr. *)
+
+Definition test : statement :=
+  <{ let A : type_int32s in
+     A#type_int32s := $1;
+     A#type_int32s := $0;
+     return (copy A#type_int32s);
+     skip; break; return0; return (move A#type_int32s);
+     if (($1) < ($0)) then
+       B#type_int32s := copy C#type_int32s;
+       A#type_int32s := copy B#type_int32s
+     else
+       A#type_int32s := copy C#type_int32s
+     end;
+     loop
+       A#type_int32s := copy C#type_int32s;
+       B#type_int32s := copy A#type_int32s
+     end;
+     return0
+     end }>.
+
+(** ** Pretty printing for Rustlight programs  *)
