rustfrontend/Rustlightown.v
@@ -1,0 +1,923 @@
+Require Import Coqlib.
+Require Import Errors.
+Require Import Maps.
+Require Import Integers.
+Require Import Floats.
+Require Import Values.
+Require Import AST.
+Require Import Memory.
+Require Import Events.
+Require Import Globalenvs.
+Require Import Smallstep.
+Require Import Ctypes Rusttypes Rustlight.
+Require Import Cop RustOp.
+Require Import LanguageInterface.
+Require Import InitDomain.
+
+Local Open Scope error_monad_scope.
+
+
+(** Generate drop glue map like RustIR *)
+
+
+(* Extract composite id to drop glue id list *)
+Definition extract_drop_id (g: ident * globdef fundef type) : ident * ident :=
+  let (glue_id, def) := g in
+  match def with
+  | Gfun (Internal f) =>
+      match f.(fn_drop_glue) with
+      | Some comp_id => (comp_id, glue_id)
+      | None => (1%positive, glue_id)
+      end
+  | _ => (1%positive, glue_id)
+  end.
+
+Definition check_drop_glue (g: ident * globdef fundef type) : bool :=
+  let (glue_id, def) := g in
+  match def with
+  | Gfun (Internal f) =>
+      match f.(fn_drop_glue) with
+      | Some comp_id => true
+      | None => false
+      end
+  | _ => false
+  end.
+
+Definition generate_dropm (p: program) :=
+  let drop_glue_ids := map extract_drop_id (filter check_drop_glue p.(prog_defs)) in
+  PTree_Properties.of_list drop_glue_ids.
+
+
+(** * Operational Semantics  *)
+
+(** ** Global environment  *)
+
+Record genv := { genv_genv :> Genv.t fundef type; genv_cenv :> composite_env; genv_dropm :> PTree.t ident }.
+  
+Definition globalenv (se: Genv.symtbl) (p: program) :=
+  {| genv_genv := Genv.globalenv se p; genv_cenv := p.(prog_comp_env); genv_dropm := generate_dropm p |}.
+
+(** ** Local environment  *)
+
+Definition env := PTree.t (block * type). (* map variable -> location & type *)
+
+Definition empty_env: env := (PTree.empty (block * type)).
+
+(** ** Ownership environment  *)
+
+
+(** Ownership environment: a pair of deep owned place set and
+shallow owned place set (TODO: it should be defined in Rustlight) *)
+    
+(** own_env is actually init environment which is used to check
+every used is initialized. Maybe we should change the name?  *)
+
+(* may be we can use PathMap to optimize it *)
+Record own_env :=
+  mkown { own_init: PathsMap.t;
+          own_uninit: PathsMap.t;
+          own_universe: PathsMap.t } .
+
+Definition is_owned (own: own_env) (p: place): bool :=
+  let id := local_of_place p in
+  let init := PathsMap.get id own.(own_init) in
+  let uninit := PathsMap.get id own.(own_uninit) in
+  (* no p's prefix in uninit and there is some p's prefix in init *)
+  Paths.for_all (fun p' => negb (is_prefix p' p)) uninit
+  && Paths.exists_ (fun p' => is_prefix p' p) init.
+
+(* A owned place is deep owned **xor** shallow owned *)
+
+Definition is_deep_owned (own: own_env) (p: place) : bool :=
+  (* p is owned and no p's children in the universe *)
+  is_owned own p &&
+    let id := local_of_place p in
+    let universe := PathsMap.get id own.(own_universe) in
+    Paths.for_all (fun p' => negb (is_prefix_strict p p')) universe.
+
+Definition is_shallow_owned (own: own_env) (p: place) : bool :=
+  is_owned own p &&
+    (* There is some p's children in the universe, which means that
+    p's ownership may be split. So we only consider p as a partial
+    owned place *)
+    let id := local_of_place p in
+    let universe := PathsMap.get id own.(own_universe) in
+    Paths.exists_ (fun p' => is_prefix_strict p p') universe.
+
+(* check that parents of p are not in uninit (slightly different from
+   the condition in is_owned) *)
+Definition prefix_is_owned (own: own_env) (p: place) : bool :=
+  forallb (is_owned own) (parent_paths p).
+  (* let id := local_of_place p in *)
+  (* let uninit := PathsMap.get id own.(own_uninit) in *)
+  (* (* no p's prefix in uninit *) *)
+  (* Paths.for_all (fun p' => negb (is_prefix_strict p' p)) uninit. *)
+
+Lemma prefix_owned_implies: forall p p' own,
+    prefix_is_owned own p = true ->
+    is_prefix_strict p' p = true ->
+    is_owned own p' = true.
+Proof.
+  intros p p' own POWN PFX.
+  eapply forallb_forall in POWN; eauto.
+  eapply proj_sumbool_true in PFX. auto.
+Qed.  
+  
+(* place with succesive Pdowncast in the end is not a valid owner. For
+example, move (Pdowncast p) is equivalent to move p *)
+Fixpoint valid_owner (p: place) :=
+  match p with
+  | Pdowncast p' _ _ => valid_owner p'
+  | _ => p
+  end.
+
+Definition check_movable (own: own_env) (p: place) : bool :=
+  (* the place itself and its children are all owned *)
+  let id := local_of_place p in
+  let universe := PathsMap.get id (own_universe own) in  
+  Paths.for_all (is_owned own) (Paths.filter (is_prefix p) universe).
+
+
+Fixpoint own_check_pexpr (own: own_env) (pe: pexpr) : bool :=
+  match pe with
+  | Eplace p _
+  | Ecktag p _
+  | Eref _ _ p _ =>
+      (* we only check p which represents/owns a memory location *)
+      if place_owns_loc p then
+        (* copy/reference a place also requires that the place is
+        movable (all its children are owned, otherwise it is not
+        memory safe because the unowned block may be deallocated *)
+        check_movable own p
+      else
+        (* This checking is left for borrow checker *)
+        true
+  | Eunop _ pe _ =>
+      own_check_pexpr own pe
+  | Ebinop _ pe1 pe2 _ =>
+      own_check_pexpr own pe1 && own_check_pexpr own pe2
+  | _ => true
+end.          
+
+Definition move_place (own: own_env) (p: place) : own_env :=
+  (mkown (remove_place p own.(own_init))
+     (add_place own.(own_universe) p own.(own_uninit))
+     own.(own_universe)).
+
+
+(* Move to Rustlight: Check the ownership of expression *)
+Definition own_check_expr (own: own_env) (e: expr) : option own_env :=
+  match e with
+  | Emoveplace p ty =>
+      (** FIXME: when to use valid_owner? *)
+      let p := valid_owner p in
+      if check_movable own p then
+        (* consider [a: Box<Box<Box<i32>>>] and we move [*a]. [a] becomes
+        partial owned *)
+        (* remove p from init and add p and its children to uninit *)
+        Some (move_place own p)
+      else
+        (* Error! We must move a movable place! *)
+        None
+  | Epure pe =>
+      if own_check_pexpr own pe then
+        Some own
+      else None
+  end.
+
+Fixpoint own_check_exprlist (own: own_env) (l: list expr) : option own_env :=
+  match l with
+  | nil => Some own
+  | e :: l' =>
+      match own_check_expr own e with
+      | Some own1 =>
+          own_check_exprlist own1 l'
+      | None => None
+      end
+  end.
+
+(* The dominator of a place [p]: the place's demonator decide the
+location of this place *)
+
+Fixpoint place_dominator (p: place) : option place :=
+  match p with
+  | Pderef p' _ => Some p'
+  | Pfield p' _ _ => place_dominator p'
+  | Pdowncast p' _ _ => Some p'
+  | Plocal _ _ => None
+  end.
+
+(* A place's dominator is owned means that this place is the owner of
+the location it resides in *)
+Definition place_dominator_own (own: own_env) (p: place) : bool :=
+  match place_dominator p with
+  | Some p' => is_owned own p'
+  | None => true
+  end.
+
+(* We can use the following function to ensure that the block place
+[p] resides in is in the domain of abstracter *)
+Definition place_dominator_shallow_own (own: own_env) (p: place) : bool :=
+  match place_dominator p with
+  | Some p' => is_shallow_owned own p'
+  | None => true
+  end.
+
+
+(* Update the ownership environment when assigning to p. We must
+ensure that p is not deeply owned because p must be dropped before
+this assignment. *)
+Definition own_check_assign (own: own_env) (p: place) : option own_env :=
+  (* check that the dominator of p is owned (initialized) because we
+  need to compute the address of [p] *)
+  if place_dominator_own own p then
+    Some (mkown (add_place own.(own_universe) p own.(own_init))
+            (remove_place p own.(own_uninit))
+            own.(own_universe))
+  else
+    None.             
+
+(** Deference a location based on the type  *)
+
+Inductive deref_loc (ty: type) (m: mem) (b: block) (ofs: ptrofs) : val -> Prop :=
+  | deref_loc_value: forall chunk v,
+      access_mode ty = By_value chunk ->
+      Mem.loadv chunk m (Vptr b ofs) = Some v ->
+      deref_loc ty m b ofs v
+  | deref_loc_reference:
+      access_mode ty = By_reference ->
+      deref_loc ty m b ofs (Vptr b ofs)
+  | deref_loc_copy:
+      access_mode ty = By_copy ->
+      deref_loc ty m b ofs (Vptr b ofs).
+
+(** Memory error in deref_loc  *)
+
+Inductive deref_loc_mem_error (ty: type) (m: mem) (b: block) (ofs: ptrofs) : Prop :=
+  | deref_loc_value_error: forall chunk,
+      access_mode ty = By_value chunk ->
+      ~ Mem.valid_access m chunk b (Ptrofs.unsigned ofs) Readable ->
+      deref_loc_mem_error ty m b ofs.
+
+
+(** Assign a value to a location  *)
+
+Inductive assign_loc (ce: composite_env) (ty: type) (m: mem) (b: block) (ofs: ptrofs): val -> mem -> Prop :=
+  | assign_loc_value: forall v chunk m',
+      access_mode ty = By_value chunk ->
+      Mem.storev chunk m (Vptr b ofs) v = Some m' ->
+      assign_loc ce ty m b ofs v m'
+  | assign_loc_copy: forall b' ofs' bytes m',
+      access_mode ty = By_copy ->
+      complete_type ce ty = true ->
+      (* consider a = b ( a and b are struct ) *)
+      (* evaluate b is (Vptr b' ofs'), evaluate a is (b,ofs) *)      
+      (sizeof ce ty > 0 -> (alignof_blockcopy ce ty | Ptrofs.unsigned ofs')) ->
+      (sizeof ce ty > 0 -> (alignof_blockcopy ce ty | Ptrofs.unsigned ofs)) ->
+      (* a and b are disjoint or equal *)
+      b' <> b \/ Ptrofs.unsigned ofs' = Ptrofs.unsigned ofs
+             \/ Ptrofs.unsigned ofs' + sizeof ce ty <= Ptrofs.unsigned ofs
+             \/ Ptrofs.unsigned ofs + sizeof ce ty <= Ptrofs.unsigned ofs' ->
+      Mem.loadbytes m b' (Ptrofs.unsigned ofs') (sizeof ce ty) = Some bytes ->
+      Mem.storebytes m b (Ptrofs.unsigned ofs) bytes = Some m' ->
+      assign_loc ce ty m b ofs (Vptr b' ofs') m'.
+
+(** Memory error in assign_loc  *)
+
+Inductive assign_loc_mem_error (ce : composite_env) (ty : type) (m : mem) (b : block) (ofs : ptrofs) : val -> Prop :=
+| assign_loc_value_mem_error: forall v chunk,
+    access_mode ty = By_value chunk ->
+    ~ Mem.valid_access m chunk b (Ptrofs.unsigned ofs) Writable ->
+    assign_loc_mem_error ce ty m  b ofs v
+| assign_loc_copy_mem_error1: forall b' ofs',
+    (* the memory location of the struct to be copied is not readable *)
+    access_mode ty = By_copy ->
+    ~ Mem.range_perm m b' (Ptrofs.unsigned ofs') ((Ptrofs.unsigned ofs') + (sizeof ce ty)) Cur Readable ->
+    assign_loc_mem_error ce ty m b ofs (Vptr b' ofs')
+| assign_loc_copy_mem_error2: forall v,
+    (* the memory location of the struct to be stored is not writable *)
+    access_mode ty = By_copy ->
+    Mem.range_perm m b (Ptrofs.unsigned ofs) ((Ptrofs.unsigned ofs) + (sizeof ce ty)) Cur Writable ->
+    assign_loc_mem_error ce ty m b ofs v.
+
+
+Section SEMANTICS.
+  
+(** ** Evaluation of expressions *)
+
+Section EXPR.
+
+Variable ce: composite_env.
+Variable e: env.
+Variable m: mem.
+
+(* similar to eval_lvalue in Clight.v *)
+Inductive eval_place : place -> block -> ptrofs -> Prop :=
+| eval_Plocal: forall id b ty,
+    (** TODO: there is no global variable, so we do not consider the
+    gloabl environment *)
+    e!id = Some (b, ty) ->
+    eval_place (Plocal id ty) b Ptrofs.zero
+| eval_Pfield_struct: forall p ty b ofs delta id i co orgs,
+    eval_place p b ofs ->
+    typeof_place p = Tstruct orgs id ->
+    ce ! id = Some co ->
+    field_offset ce i (co_members co) = OK delta ->
+    eval_place (Pfield p i ty) b (Ptrofs.add ofs (Ptrofs.repr delta))
+| eval_Pdowncast: forall  p ty b ofs fofs id fid fty co orgs tag,
+    eval_place p b ofs ->
+    typeof_place p = Tvariant orgs id ->
+    ce ! id = Some co ->
+    (* check tag and fid *)
+    Mem.loadv Mint32 m (Vptr b ofs) = Some (Vint tag) ->
+    list_nth_z co.(co_members) (Int.unsigned tag) = Some (Member_plain fid fty) ->
+    variant_field_offset ce fid (co_members co) = OK fofs ->
+    (* fty and ty must be equal? *)
+    eval_place (Pdowncast p fid ty) b (Ptrofs.add ofs (Ptrofs.repr fofs))
+| eval_Pderef: forall p ty l ofs l' ofs',
+    eval_place p l ofs ->
+    deref_loc (typeof_place p) m l ofs (Vptr l' ofs') ->
+    eval_place (Pderef p ty) l' ofs'.
+
+Inductive eval_place_mem_error : place -> Prop :=
+| eval_Pfield_error: forall p ty i,
+    eval_place_mem_error p ->
+    eval_place_mem_error (Pfield p i ty)
+| eval_Pdowncast_error1: forall p ty fid,
+    eval_place_mem_error p ->
+    eval_place_mem_error (Pdowncast p fid ty)
+| eval_Pdowncast_error2: forall p ty fid b ofs,
+    eval_place p b ofs ->
+    ~ Mem.valid_access m Mint32 b (Ptrofs.unsigned ofs) Readable ->
+    eval_place_mem_error (Pdowncast p fid ty)
+| eval_Pderef_error1: forall p ty,
+    eval_place_mem_error p ->
+    eval_place_mem_error (Pderef p ty)
+| eval_Pderef_error2: forall p l ofs ty,
+    eval_place p l ofs ->
+    deref_loc_mem_error (typeof_place p) m l ofs ->
+    eval_place_mem_error (Pderef p ty)
+.
+
+
+Inductive eval_place_list : list place -> list block -> list ptrofs -> Prop :=
+| eval_Pnil: eval_place_list nil nil nil
+| eval_Pcons: forall p b ofs lp lb lofs,
+    eval_place p b ofs ->
+    eval_place_list lp lb lofs ->    
+    eval_place_list (p :: lp) (b :: lb) (ofs :: lofs).
+
+
+Definition int_val_casted (v: val) (ty: type) : Prop :=
+  match v, ty with
+  | Vint n, Tint sz sg =>
+      cast_int_int sz sg n = n
+  | _, _ => True
+  end.
+
+
+(* Evaluation of pure expression *)
+
+Inductive eval_pexpr: pexpr -> val ->  Prop :=
+| eval_Eunit:
+    eval_pexpr Eunit (Vint Int.zero)
+| eval_Econst_int:   forall i ty,
+    eval_pexpr (Econst_int i ty) (Vint i)
+| eval_Econst_float:   forall f ty,
+    eval_pexpr (Econst_float f ty) (Vfloat f)
+| eval_Econst_single:   forall f ty,
+    eval_pexpr (Econst_single f ty) (Vsingle f)
+| eval_Econst_long:   forall i ty,
+    eval_pexpr (Econst_long i ty) (Vlong i)
+| eval_Eunop:  forall op a ty v1 v aty,
+    eval_pexpr a v1 ->
+    (* Note that to_ctype Tbox = None *)
+    to_ctype (typeof_pexpr a) = aty ->
+    (** TODO: define a rust-specific sem_unary_operation  *)
+    sem_unary_operation op v1 aty m = Some v ->
+    eval_pexpr (Eunop op a ty) v
+| eval_Ebinop: forall op a1 a2 ty v1 v2 v ty1 ty2,
+    eval_pexpr a1 v1 ->
+    eval_pexpr a2 v2 ->
+    to_ctype (typeof_pexpr a1) = ty1 ->
+    to_ctype (typeof_pexpr a2) = ty2 ->
+    sem_binary_operation_rust op v1 ty1 v2 ty2 m = Some v ->
+    (* For now, we do not return moved place in binary operation *)
+    eval_pexpr (Ebinop op a1 a2 ty) v
+| eval_Eplace: forall p b ofs ty v,
+    eval_place p b ofs ->
+    deref_loc ty m b ofs v ->
+    (* adhoc: cast int if v is Vint. This premise is only useful if ty
+    is type_bool and v is i8 which may be non-zero and non-one
+    value. But we want to prove that it is one or zero *)
+    (* int_val_casted v ty -> *)
+    eval_pexpr (Eplace p ty) v
+| eval_Ecktag: forall (p: place) b ofs tag tagz id fid co orgs,
+    eval_place p b ofs ->
+    (* load the tag *) 
+    Mem.loadv Mint32 m (Vptr b ofs) = Some (Vint tag) ->
+    typeof_place p = Tvariant orgs id ->
+    ce ! id = Some co ->
+    field_tag fid co.(co_members) = Some tagz ->
+    eval_pexpr (Ecktag p fid) (Val.of_bool (Int.eq tag (Int.repr tagz)))
+| eval_Eref: forall p b ofs mut ty org,
+    eval_place p b ofs ->
+    eval_pexpr (Eref org mut p ty) (Vptr b ofs).
+
+      
+(* expression evaluation has two phase: evaluate the value and produce
+the moved-out place *)
+Inductive eval_expr: expr -> val -> Prop :=
+| eval_Emoveplace: forall p ty v,
+    eval_pexpr (Eplace p ty) v ->
+    eval_expr (Emoveplace p ty) v
+(* | eval_Emoveget: forall p fid ty v, *)
+(*     eval_pexpr (Eget p fid ty) v -> *)
+(*     eval_expr (Emoveget p fid ty) v *)
+| eval_Epure: forall pe v,
+    eval_pexpr pe v ->
+    eval_expr (Epure pe) v.
+
+Inductive eval_exprlist : list expr -> typelist -> list val -> Prop :=
+| eval_Enil:
+  eval_exprlist nil Tnil nil
+| eval_Econs:   forall a bl ty tyl v1 v2 vl,
+    eval_expr a v1 ->
+    sem_cast v1 (typeof a) ty = Some v2 ->
+    eval_exprlist bl tyl vl ->
+    eval_exprlist (a :: bl) (Tcons ty tyl) (v2 :: vl).
+
+(** Memory error in evaluation of expression  *)
+
+
+Inductive eval_pexpr_mem_error: pexpr ->  Prop :=
+| eval_Eunop_error:  forall op a ty,
+    eval_pexpr_mem_error a ->
+    eval_pexpr_mem_error (Eunop op a ty)
+| eval_Ebinop_error: forall op a1 a2 ty,
+    (eval_pexpr_mem_error a1 \/ eval_pexpr_mem_error a2) ->
+    eval_pexpr_mem_error (Ebinop op a1 a2 ty)
+| eval_Eplace_error1: forall p ty,
+    eval_place_mem_error p ->
+    eval_pexpr_mem_error (Eplace p ty)
+| eval_Eplace_error2: forall p b ofs ty,
+    eval_place p b ofs->
+    deref_loc_mem_error ty m b ofs ->
+    eval_pexpr_mem_error (Eplace p ty)
+| eval_Ecktag_error1: forall p fid,
+    eval_place_mem_error p ->
+    eval_pexpr_mem_error (Ecktag p fid)
+| eval_Ecktag_error2: forall p b ofs fid, 
+    eval_place p b ofs ->
+    (* tag is not readable *)
+    ~ Mem.valid_access m Mint32 b (Ptrofs.unsigned ofs) Readable ->
+    eval_pexpr_mem_error (Ecktag p fid)
+| eval_Eref_error: forall p org mut ty,
+    eval_place_mem_error p ->
+    eval_pexpr_mem_error (Eref org mut p ty).
+
+Inductive eval_expr_mem_error: expr -> Prop :=
+| eval_Emoveplace_error: forall p ty,
+    eval_pexpr_mem_error (Eplace p ty) ->
+    eval_expr_mem_error (Emoveplace p ty)
+| eval_Epure_mem_error: forall pe,
+    eval_pexpr_mem_error pe ->
+    eval_expr_mem_error (Epure pe).
+
+Inductive eval_exprlist_mem_error : list expr -> typelist -> Prop :=
+| eval_Econs_mem_error1: forall a bl ty tyl,
+    eval_expr_mem_error a ->
+    eval_exprlist_mem_error (a :: bl) (Tcons ty tyl)
+| eval_Econs_mem_error2: forall a bl ty tyl v1,
+    eval_expr a v1 ->
+    eval_exprlist_mem_error bl tyl ->
+    eval_exprlist_mem_error (a :: bl) (Tcons ty tyl)
+.
+
+
+End EXPR.
+
+
+(** Continuations *)
+
+Inductive cont : Type :=
+| Kstop: cont
+| Kseq: statement -> cont -> cont
+| Klet: ident -> cont -> cont
+| Kloop: statement -> cont -> cont
+| Kcall: place  -> function -> env -> own_env -> cont -> cont.
+
+
+(** Pop continuation until a call or stop *)
+
+Fixpoint call_cont (k: cont) : cont :=
+  match k with
+  | Kseq s k => call_cont k
+  | Kloop s k => call_cont k
+  (* pop Klet *)
+  | Klet id k => call_cont k
+  | _ => k
+  end.
+
+Definition is_call_cont (k: cont) : Prop :=
+  match k with
+  | Kstop => True
+  | Kcall _ _ _ _ _ => True
+  | _ => False
+  end.
+
+(** States *)
+
+Inductive state: Type :=
+  | State
+      (f: function)
+      (s: statement)
+      (k: cont)
+      (e: env)
+      (ie: own_env)
+      (m: mem) : state
+  | Callstate
+      (vf: val)
+      (args: list val)
+      (k: cont)
+      (m: mem) : state
+  | Returnstate
+      (res: val)
+      (k: cont)
+      (m: mem) : state.                          
+
+
+(** Allocate memory blocks for function parameters/variables and build
+the local environment *)
+Inductive alloc_variables (ce: composite_env) : env -> mem ->
+                                                list (ident * type) ->
+                                                env -> mem -> Prop :=
+| alloc_variables_nil:
+  forall e m,
+    alloc_variables ce e m nil e m
+| alloc_variables_cons:
+  forall e m id ty vars m1 b1 m2 e2,
+    Mem.alloc m 0 (sizeof ce ty) = (m1, b1) ->
+    alloc_variables ce (PTree.set id (b1, ty) e) m1 vars e2 m2 ->
+    alloc_variables ce e m ((id, ty) :: vars) e2 m2.
+
+(** Assign the values to the memory blocks of the function parameters  *)
+Inductive bind_parameters (ce: composite_env) (e: env):
+                           mem -> list (ident * type) -> list val ->
+                           mem -> Prop :=
+  | bind_parameters_nil:
+      forall m,
+      bind_parameters ce e m nil nil m
+  | bind_paranmeters_cons:
+      forall m id ty params v1 vl b m1 m2,
+      PTree.get id e = Some(b, ty) ->
+      assign_loc ce ty m b Ptrofs.zero v1 m1 ->
+      bind_parameters ce e m1 params vl m2 ->
+      bind_parameters ce e m ((id, ty) :: params) (v1 :: vl) m2.
+
+Inductive bind_parameters_mem_error (ce: composite_env) (e: env) : mem -> list (ident * type) -> list val -> Prop :=
+| bind_parameters_mem_error_cons1: forall m id ty params v1 vl b,
+    e ! id = Some (b, ty) ->
+    assign_loc_mem_error ce ty m b Ptrofs.zero v1 ->
+    bind_parameters_mem_error ce e m ((id, ty) :: params) (v1 :: vl)
+| bind_parameters_mem_error_cons2: forall m id ty params v1 vl b m1,
+    e ! id = Some (b, ty) ->
+    assign_loc ce ty m b Ptrofs.zero v1 m1 ->
+    bind_parameters_mem_error ce e m1 params vl ->
+    bind_parameters_mem_error ce e m ((id, ty) :: params) (v1 :: vl).
+
+
+(** Return the list of blocks in the codomain of [e], with low and high bounds. *)
+
+Definition block_of_binding (ce: composite_env) (id_b_ty: ident * (block * type)) :=
+  match id_b_ty with (id, (b, ty)) => (b, 0, sizeof ce ty) end.
+
+Definition blocks_of_env (ce: composite_env) (e: env) : list (block * Z * Z) :=
+  List.map (block_of_binding ce) (PTree.elements e).
+
+(** Return the list of places in local environment  *)
+
+Definition place_of_binding (id_b_ty: ident * (block * type)) :=
+  match id_b_ty with (id, (b, ty)) => (Plocal id ty) end.
+
+Definition places_of_env (e:env) : list place :=
+  List.map place_of_binding (PTree.elements e).
+
+
+(* Some functions used in generating initial own environment *)
+
+Section WITH_CE.
+
+Variable ce: composite_env.
+
+Fixpoint collect_stmt (s: statement) (m: PathsMap.t) : PathsMap.t :=
+  match s with
+  | Sassign_variant p _ _ e
+  | Sassign p e
+  | Sbox p e =>
+      collect_place ce p (collect_expr ce e m)
+  | Scall p _ al =>
+      collect_place ce p (collect_exprlist ce al m)
+  | Sreturn (Some e) =>
+      collect_expr ce e m
+  | Ssequence s1 s2 =>
+      collect_stmt s1 (collect_stmt s2 m)
+  | Sifthenelse e s1 s2 =>
+      collect_stmt s1 (collect_stmt s2 (collect_expr ce e m))
+  | Sloop s =>
+      collect_stmt s m
+  | _ => m
+  end.
+
+Definition collect_func (f: function) : Errors.res PathsMap.t :=
+  let vars := f.(fn_params) ++ extract_vars f.(fn_body) in  
+  if list_norepet_dec ident_eq (map fst vars) then
+    let l := map (fun elt => (Plocal (fst elt) (snd elt))) vars in
+    (** TODO: add all the parameters and variables to l (may be useless?) *)
+    let init_map := fold_right (collect_place ce) (PTree.empty LPaths.t) l in
+    Errors.OK (collect_stmt f.(fn_body) init_map)
+  else
+    Errors.Error (MSG "Repeated identifiers in variables and parameters: collect_func" :: nil).
+
+End WITH_CE.
+
+(* copy from init analysis *)
+Definition init_own_env (ce: composite_env) (f: function) : Errors.res own_env :=
+  (* collect the whole set in order to simplify the gen and kill operation *)
+  do whole <- collect_func ce f;
+  (* initialize maybeInit set with parameters *)
+  let pl := map (fun elt => Plocal (fst elt) (snd elt)) f.(fn_params) in
+  (* It is necessary because we have to guarantee that the map is not
+  PathMap.bot in the 'transfer' function *)
+  let empty_pathmap := PTree.map (fun _ elt => Paths.empty) whole in
+  let init := fold_right (add_place whole) empty_pathmap pl in
+  (* initialize maybeUninit with the variables *)
+  let vl := map (fun elt => Plocal (fst elt) (snd elt)) (extract_vars f.(fn_body)) in
+  let uninit := fold_right (add_place whole) empty_pathmap vl in
+  OK (mkown init uninit whole).
+
+(* Use extract_vars to extract the local variables *)
+
+Inductive function_entry (ge: genv) (f: function) (vargs: list val) (m: mem) (e: env) (m2: mem) (own: own_env) : Prop :=
+| function_entry_intro: forall m1 vars
+    (VARS: vars = extract_vars f.(fn_body))
+    (NOREP: list_norepet (var_names f.(fn_params) ++ var_names vars))
+    (ALLOC: alloc_variables ge empty_env m (f.(fn_params) ++ vars) e m1)
+    (BIND: bind_parameters ge e m1 f.(fn_params) vargs m2)
+    (* initialize own_env *)
+    (INITOWN: init_own_env ge f = OK own),
+    function_entry ge f vargs m e m2 own.
+
+
+Section SMALLSTEP.
+
+Variable ge: genv.
+
+Inductive step : state -> trace -> state -> Prop :=
+
+| step_assign: forall f e (p: place) ty op k le own own' own'' m1 m2 m3 b ofs v id  orgs,
+    (** FIXME: some ugly restriction  *)
+    typeof_place p = ty ->
+    typeof e = ty ->
+    ty <> Tvariant orgs id  ->
+    (* get the location of the place *)
+    eval_place ge le m1 p b ofs ->
+    (* evaluate the expr, return the value and the moved place (optional) *)
+    eval_expr ge le m1 e v ->
+    moved_place e = op ->
+    (* update the initialized environment based on [op] *)
+    remove_own_option own op = Some own' ->
+    (* drop the successors of p (i.e., *p, **p, ...). If ty is not
+    owned type, drop_place has no effect. We must first update the me
+    and then drop p, consider [ *p=move *p ] *)
+    drop_place ge le own' p m1 m2 ->
+    (* update the ownership env for p *)
+    PTree.set (local_of_place p) (own_path ge p (typeof_place p)) own' = own'' ->
+    (* assign to p  *)
+    (* note that the type is the expreesion type, consider [a = 1]
+    where a is [variant{int,float} *)
+    assign_loc ge ty m2 b ofs v m3 ->
+    step (State f (Sassign p e) k le own m1) E0 (State f Sskip k le own'' m3) 
+         
+| step_assign_variant: forall f e (p: place) ty op k le own own' own'' m1 m2 m3 m4 b ofs ofs' v tag co id fid enum_id  orgs,
+    typeof_place p = ty ->
+    typeof e = ty ->
+    ty = Tvariant orgs id  ->
+    (* get the location of the place *)
+    eval_place ge le m1 p b ofs ->
+    (* evaluate the boxexpr, return the value and the moved place (optional) *)
+    eval_expr ge le m1 e v ->
+    moved_place e = op ->
+    (* update the initialized environment based on [op] *)
+    remove_own_option own op = Some own' ->
+    (* drop the successors of p (i.e., *p, **p, ...). If ty is not
+    owned type, drop_place has no effect. We must first update the me
+    and then drop p, consider [ *p=move *p ] *)
+    drop_place ge le own' p m1 m2 ->
+    (* update the ownership env for p *)
+    PTree.set (local_of_place p) (own_path ge p (typeof_place p)) own' = own'' ->
+    (* assign to p  *)
+    (** different from normal assignment: update the tag and assign value *)
+    ge.(genv_cenv) ! id = Some co ->
+    field_tag fid co.(co_members) = Some tag ->
+    (* set the tag *)
+    Mem.storev Mint32 m2 (Vptr b ofs) (Vint (Int.repr tag)) = Some m3 ->
+    field_offset ge fid co.(co_members) = OK ofs' ->
+    (* set the value *)
+    assign_loc ge ty m3 b (Ptrofs.add ofs (Ptrofs.repr ofs')) v m4 ->
+    step (State f (Sassign_variant p enum_id fid e) k le own m1) E0 (State f Sskip k le own'' m4)
+
+| step_box: forall f e (p: place) ty op k le own1 own2 own3 m1 m2 m3 b v,
+    typeof e = ty ->
+    (* typeof_place p = TSletbox ty attr -> *)
+    eval_expr ge le m1 e v ->
+    (* allocate the memory block *)
+    Mem.alloc m1 0 (sizeof ge ty) = (m2, b) ->
+    (* assign the value *)
+    assign_loc ge ty m2 b Ptrofs.zero v m3 ->
+    (* update the ownership environment *)
+    moved_place e = op ->
+    remove_own_option own1 op = Some own2 ->
+    (* update the ownership env for p *)
+    PTree.set (local_of_place p) (own_path ge p ty) own2 = own3 ->
+    step (State f (Sbox p e) k le own1 m1) E0 (* may be we can change the effect *) (State f Sskip k le own3 m3)  
+         
+| step_let: forall f ty id own m1 m2 le1 le2 b k stmt,
+    (* allocate the block for id *)
+    Mem.alloc m1 0 (sizeof ge ty) = (m2, b) ->
+    (* uppdate the local env *)
+    PTree.set id (b, ty) le1 = le2 ->
+    step (State f (Slet id ty stmt) k le1 own m1) E0 (State f stmt (Klet id k) le2 own m2)
+
+         
+(** FIXME: we do not allow initialization in let statement. So that we
+can initialize struct *)
+(* | step_let: forall f be op v ty id own1 own2 own3 m1 m2 m3 m4 le1 le2 b k stmt, *)
+(*     typeof_boxexpr be = ty -> *)
+(*     eval_boxexpr ge le1 m1 be v op m2 -> *)
+(*     (* update the move environment *) *)
+(*     remove_own own1 op = Some own2 -> *)
+(*     (* allocate the block for id *) *)
+(*     Mem.alloc m2 0 (sizeof ge ty) = (m3, b) -> *)
+(*     (* uppdate the local env *) *)
+(*     PTree.set id (b, ty) le1 = le2 -> *)
+(*     (* update the ownership environment *) *)
+(*     PTree.set id (own_path ge (Plocal id ty) ty) own2 = own3 -> *)
+(*     (* assign [v] to [b] *) *)
+(*     assign_loc ge ty m3 b Ptrofs.zero v m4 -> *)
+(*     step (State f (Slet id ty be stmt) k le1 own1 m1) E0 (State f stmt (Klet id k) le2 own3 m3) *)
+         
+(* | step_call_0: forall f a al optlp k le own1 own2 m vargs tyargs vf fd cconv tyres, *)
+(*     classify_fun (typeof a) = fun_case_f tyargs tyres cconv -> *)
+(*     eval_expr ge le m a vf -> *)
+(*     eval_exprlist ge le m al tyargs vargs -> *)
+(*     moved_place_list al = optlp -> *)
+(*     (* CHECKME: update the initialized environment *) *)
+(*     remove_own_list own1 optlp = Some own2 -> *)
+(*     Genv.find_funct ge vf = Some fd -> *)
+(*     type_of_fundef fd = Tfunction tyargs tyres cconv -> *)
+(*     step (State f (Scall None a al) k le own1 m) E0 (Callstate vf vargs (Kcall None f le own2 k) m) *)
+| step_call_1: forall f a al optlp k le own1 own2 m vargs tyargs vf fd cconv tyres p orgs org_rels,
+    classify_fun (typeof a) = fun_case_f tyargs tyres cconv ->
+    eval_expr ge le m a vf ->
+    eval_exprlist ge le m al tyargs vargs ->
+    moved_place_list al = optlp ->
+    (* CHECKME: update the move environment *)
+    remove_own_list own1 optlp = Some own2 ->
+    Genv.find_funct ge vf = Some fd ->
+    type_of_fundef fd = Tfunction orgs org_rels tyargs tyres cconv ->
+    step (State f (Scall p a al) k le own1 m) E0 (Callstate vf vargs (Kcall p f le own2 k) m)
+                 
+(* End of a let statement, free the place and its drop obligations *)
+| step_end_let: forall f id k le1 le2 own1 own2 m1 m2 m3 ty b s,
+    s = Sskip \/ s = Sbreak \/ s = Scontinue ->
+    PTree.get id le1 = Some (b, ty) ->
+    (* free {*id, **id, ...} if necessary *)
+    drop_place ge le1 own1 (Plocal id ty) m1 m2 ->
+    (* free the block [b] of the local variable *)
+    Mem.free m1 b 0 (sizeof ge ty) = Some m2 ->
+    (* clear [id] in the local env and move env. It is necessary for the memory deallocation in return state *)
+    PTree.remove id le1 = le2 ->
+    PTree.remove id own1 = own2 ->
+    step (State f s (Klet id k) le1 own1 m1) E0 (State f s k le2 own2 m3)
+
+| step_internal_function: forall vf f vargs k m e me m'
+    (FIND: Genv.find_funct ge vf = Some (Internal f)),
+    function_entry ge f vargs m e me m' ->
+    step (Callstate vf vargs k m) E0 (State f f.(fn_body) k e me m')
+
+| step_external_function: forall vf vargs k m m' cc ty typs ef v t orgs org_rels
+    (FIND: Genv.find_funct ge vf = Some (External orgs org_rels ef typs ty cc)),
+    external_call ef ge vargs m t v m' ->
+    step (Callstate vf vargs k m) t (Returnstate v k m')
+
+(** Return cases  *)
+| step_return_0: forall e own lp lb m1 m2 f k ,
+    places_of_env e = lp ->
+    (* drop the lived drop obligations *)
+    drop_place_list ge e own m1 lp m2 ->
+    blocks_of_env ge e = lb ->
+    (* drop the stack blocks *)
+    Mem.free_list m1 lb = Some m2 ->
+    step (State f (Sreturn None) k e own m1) E0 (Returnstate Vundef (call_cont k) m2)
+| step_return_1: forall le a v op own own' lp lb m1 m2 m3 f k ,
+    eval_expr ge le m1 a v ->
+    moved_place a = op ->
+    (* CHECKME: update move environment, because some place may be
+    moved out to the callee *)
+    remove_own_option own op = Some own' ->
+    places_of_env le = lp ->
+    drop_place_list ge le own' m1 lp m2 ->
+    (* drop the stack blocks *)
+    blocks_of_env ge le = lb ->
+    Mem.free_list m2 lb = Some m3 ->
+    step (State f (Sreturn (Some a)) k le own m1) E0 (Returnstate v (call_cont k) m3)
+(* no return statement but reach the end of the function *)
+| step_skip_call: forall e own lp lb m1 m2 m3 f k,
+    is_call_cont k ->
+    places_of_env e = lp ->
+    drop_place_list ge e own m1 lp m2 ->
+    blocks_of_env ge e = lb ->
+    Mem.free_list m2 lb = Some m3 ->
+    step (State f Sskip k e own m1) E0 (Returnstate Vundef (call_cont k) m3)
+         
+(* | step_returnstate_0: forall v m e me f k, *)
+(*     step (Returnstate v (Kcall None f e me k) m) E0 (State f Sskip k e me m) *)
+| step_returnstate_1: forall (p: place) v b ofs ty m m' m'' e own own' f k,
+    (* drop and replace *)
+    drop_place ge e own p m m' ->
+    (* update the ownership environment *)
+    PTree.set (local_of_place p) (own_path ge p (typeof_place p)) own = own' ->
+    eval_place ge e m' p b ofs ->
+    assign_loc ge ty m' b ofs v m'' ->    
+    step (Returnstate v (Kcall p f e own k) m) E0 (State f Sskip k e own' m'')
+
+(* Control flow statements *)
+| step_seq:  forall f s1 s2 k e me m,
+    step (State f (Ssequence s1 s2) k e me m)
+      E0 (State f s1 (Kseq s2 k) e me m)
+| step_skip_seq: forall f s k e me m,
+    step (State f Sskip (Kseq s k) e me m)
+      E0 (State f s k e me m)
+| step_continue_seq: forall f s k e me m,
+    step (State f Scontinue (Kseq s k) e me m)
+      E0 (State f Scontinue k e me m)
+| step_break_seq: forall f s k e me m,
+    step (State f Sbreak (Kseq s k) e me m)
+      E0 (State f Sbreak k e me m)
+| step_ifthenelse:  forall f a s1 s2 k e me me' m v1 b ty,
+    (* there is no receiver for the moved place, so it must be None *)
+    eval_expr ge e m a v1 ->
+    to_ctype (typeof a) = ty ->
+    bool_val v1 ty m = Some b ->
+    step (State f (Sifthenelse a s1 s2) k e me m)
+      E0 (State f (if b then s1 else s2) k e me' m)
+| step_loop: forall f s k e me m,
+    step (State f (Sloop s) k e me m)
+      E0 (State f s (Kloop s k) e me m)
+| step_skip_or_continue_loop:  forall f s k e me m x,
+    x = Sskip \/ x = Scontinue ->
+    step (State f x (Kloop s k) e me m)
+      E0 (State f s (Kloop s k) e me m)
+| step_break_loop:  forall f s k e me m,
+    step (State f Sbreak (Kloop s k) e me m)
+      E0 (State f Sskip k e me m)
+.
+
+
+(** Open semantics *)
+
+(** IDEAS: can we check the validity of the input values based on the
+function types?  *)
+Inductive initial_state: c_query -> state -> Prop :=
+| initial_state_intro: forall vf f targs tres tcc ctargs ctres vargs m orgs org_rels,
+    Genv.find_funct ge vf = Some (Internal f) ->
+    type_of_function f = Tfunction orgs org_rels targs tres tcc ->
+    (** TODO: val_casted_list *)
+    Mem.sup_include (Genv.genv_sup ge) (Mem.support m) ->
+    initial_state (cq vf (signature_of_type ctargs ctres tcc) vargs m)
+                  (Callstate vf vargs Kstop m).
+    
+Inductive at_external: state -> c_query -> Prop:=
+| at_external_intro: forall vf name sg args k m targs tres cconv orgs org_rels,
+    Genv.find_funct ge vf = Some (External orgs org_rels (EF_external name sg) targs tres cconv) ->    
+    at_external (Callstate vf args k m) (cq vf sg args m).
+
+Inductive after_external: state -> c_reply -> state -> Prop:=
+| after_external_intro: forall vf args k m m' v,
+    after_external
+      (Callstate vf args k m)
+      (cr v m')
+      (Returnstate v k m').
+
+Inductive final_state: state -> c_reply -> Prop:=
+| final_state_intro: forall v m,
+    final_state (Returnstate v Kstop m) (cr v m).
+
+End SMALLSTEP.
+
+End SEMANTICS.
+
+Definition semantics (p: program) :=
+  Semantics_gen step initial_state at_external (fun _ => after_external) (fun _ => final_state) globalenv p.
+
